Got a valid interpretation of jctc6

EventStructures.thy
@@ -7,7 +7,7 @@ begin
   
 (*text{* Primitive conflict has no edges in it which can be inferred by the rule 
 @{thm [source] confOverPO_def}. *}
-definition minimal :: "'a rel \<Rightarrow> 'a rel \<Rightarrow> bool" where
+definition minimal :: "event rel \<Rightarrow> event rel \<Rightarrow> bool" where
 "minimal po conf \<equiv> 
   (\<forall>w.\<forall>x.\<forall>y.\<forall>z. 
     ((y, z) \<in> conf \<and> 
@@ -19,7 +19,7 @@ definition minimal :: "'a rel \<Rightarrow> 'a rel \<Rightarrow> bool" where
 (*
 text{* Valid event structures are finite, have valid @{term primitive_order}, and valid 
 @{term primitive_conflict} *}
-definition isValid :: "'a set \<Rightarrow> 'a rel  \<Rightarrow> 'a rel \<Rightarrow> bool" where
+definition isValid :: "event set \<Rightarrow> event rel  \<Rightarrow> event rel \<Rightarrow> bool" where
 "isValid es po conf \<equiv> (
   finite es \<and>
   isValidPO es po \<and>
@@ -30,7 +30,7 @@ definition isValid :: "'a set \<Rightarrow> 'a rel  \<Rightarrow> 'a rel \<Right
 
 declare isValid_def [simp]
 
-definition isValidES :: "'a event_structure \<Rightarrow> bool" where
+definition isValidES :: "event event_structure \<Rightarrow> bool" where
 -- {* Need symmetric closure of primitive conflict *}
 "isValidES es \<equiv> isValid 
   (event_set es)
@@ -56,51 +56,51 @@ print_locale labelledES
 context labelledES
   begin     
     (*All read events in a configuration are justified by an event in that configuration*)
-    definition justified :: "'a config \<Rightarrow> bool" where
+    definition justified :: "event config \<Rightarrow> bool" where
       "justified c \<equiv> (\<forall>r\<in> c. (getMemAction (label r) = R) \<longrightarrow> 
         (\<exists>e\<in>c. (justifies_event (label e) (label r))))"
     
-    definition prec :: "'a \<Rightarrow> 'a \<Rightarrow> bool" (infixl "\<preceq>" 50) where 
+    definition prec :: "event \<Rightarrow> event \<Rightarrow> bool" (infixl "\<preceq>" 50) where 
       "prec x y \<equiv> (x, y) \<in> preceeds"
     declare prec_def[simp]
   
-    definition conf :: "'a \<Rightarrow> 'a \<Rightarrow> bool" ("#" 50) where
+    definition conf :: "event \<Rightarrow> event \<Rightarrow> bool" ("#" 50) where
       "conf x y \<equiv> (x, y) \<in> conflict"
       
-    definition conflict_free :: "'a config \<Rightarrow> bool" where
+    definition conflict_free :: "event config \<Rightarrow> bool" where
       "conflict_free C \<equiv> \<forall>x y. x \<in> C \<and> y \<in> C \<longrightarrow> \<not> conf x y"
       
-    definition down_closed :: "'a config \<Rightarrow> bool" where
+    definition down_closed :: "event config \<Rightarrow> bool" where
       "down_closed C \<equiv> \<forall>x y . x \<in> C \<and> y \<preceq> x \<longrightarrow> y \<in> C"
     
-    definition is_read :: "'a \<Rightarrow> bool" where
+    definition is_read :: "event \<Rightarrow> bool" where
       "is_read x \<equiv> (getMemAction (label x) = R)"
 
-    definition justifies_config :: "'a config \<Rightarrow> 'a config \<Rightarrow> bool"  where
+    definition justifies_config :: "event config \<Rightarrow> event config \<Rightarrow> bool"  where
       "justifies_config A B \<equiv> \<forall>x \<in> B. is_read x \<longrightarrow> (\<exists>y \<in> A. justifies_event (label y) (label x))"
 
-    definition justifies_config_subset :: "'a config \<Rightarrow> 'a config \<Rightarrow> bool" (infixl "\<lesssim>" 60) where
+    definition justifies_config_subset :: "event config \<Rightarrow> event config \<Rightarrow> bool" (infixl "\<lesssim>" 60) where
       "justifies_config_subset A B  \<equiv> A \<subseteq> B \<and> justifies_config A B"
 
-    definition justifies_config_star ::  "'a config \<Rightarrow> 'a config \<Rightarrow> bool" (infixl "\<lesssim>\<^sup>*" 60) where
+    definition justifies_config_star ::  "event config \<Rightarrow> event config \<Rightarrow> bool" (infixl "\<lesssim>\<^sup>*" 60) where
       "justifies_config_star a b \<equiv> justifies_config_subset\<^sup>*\<^sup>* a b"
       
-    definition config_domain :: "'a config set" ("\<CC>") where
+    definition config_domain :: "event config set" ("\<CC>") where
       "config_domain \<equiv> {C . conflict_free C \<and> down_closed C}"       
         
-    definition ae_justifies :: "'a config  \<Rightarrow> 'a config \<Rightarrow> bool" where
+    definition ae_justifies :: "event config  \<Rightarrow> event config \<Rightarrow> bool" where
       "ae_justifies C D \<equiv> \<forall>C' \<in> \<CC>. (C \<lesssim>\<^sup>* C') \<longrightarrow> (\<exists>C'' \<in> \<CC>. (C' \<lesssim>\<^sup>* C'') \<and> justifies_config C'' D)"
       
-    definition ae_justifies_subset :: "'a config \<Rightarrow> 'a config \<Rightarrow> bool" (infixl "\<sqsubseteq>" 60) where
+    definition ae_justifies_subset :: "event config \<Rightarrow> event config \<Rightarrow> bool" (infixl "\<sqsubseteq>" 60) where
       "ae_justifies_subset C D \<equiv> C \<subseteq> D \<and> ae_justifies C D"
     
-    definition ae_justifies_subset_star :: "'a config \<Rightarrow> 'a config \<Rightarrow> bool" (infixl "\<sqsubseteq>\<^sup>*" 60) where
+    definition ae_justifies_subset_star :: "event config \<Rightarrow> event config \<Rightarrow> bool" (infixl "\<sqsubseteq>\<^sup>*" 60) where
       "ae_justifies_subset_star C D \<equiv> ae_justifies_subset\<^sup>*\<^sup>* C D"
     
-    definition well_justified :: "'a config  \<Rightarrow> bool" where
+    definition well_justified :: "event config  \<Rightarrow> bool" where
       "well_justified C \<equiv> (justified C) \<and> C \<in> \<CC> \<and> {}\<sqsubseteq>\<^sup>*C"
     
-    definition initialConfig :: "'a set" ("\<C>" 1000) where
+    definition initialConfig :: "event set" ("\<C>" 1000) where
       "initialConfig \<equiv> {}"
                                          
     declare initialConfig_def [simp]
