jctc6.thy
@@ -18,35 +18,7 @@ definition primitive_conflict :: "nat rel" where
 definition conflict :: "nat rel" where
   "conflict \<equiv> build_conflict primitive_conflict order"
 
-   (*   
-lemma trancl_pc_subset_constructed_pc_id: "((symmetriccl (min_prim_conflict))\<^sup>+) \<subseteq> constructed_pc \<union> Id"
-  apply(rule subrelI)
-  apply(rule trancl.induct [where ?P = "\<lambda>x y. (x,y) \<in> constructed_pc \<union> Id"])
-    apply (simp_all add: constructed_pc_def symmetriccl_def)
-  apply(simp_all add: min_prim_conflict_def)
-  apply(auto)
-  done
-
-lemma pc_subset_constructed_pc: "((symmetriccl (min_prim_conflict))\<^sup>+ - Id) \<subseteq> constructed_pc"
-  apply(rule alg_subset)
-  apply(rule trancl_pc_subset_constructed_pc_id)
-  done
-    
-lemma constructed_pc_subset_pc: "constructed_pc \<subseteq> ((symmetriccl (min_prim_conflict))\<^sup>+ - Id)"
-  apply(rule subrelI)
-  apply(simp add: symmetriccl_def constructed_pc_def)
-  apply(simp add: min_prim_conflict_def)
-  apply auto
-  done
-    
-lemma constructed_pc_correct: "((symmetriccl (min_prim_conflict))\<^sup>+ - Id) = constructed_pc"
-  apply(rule equalityI constructed_pc_subset_pc pc_subset_constructed_pc)+
-  done
-*)
-
-
-
-interpretation jctc6: labelledES 
+interpretation jctc6 : labelledES 
   "order"
   "event_set"
   "conflict" -- Conflict
@@ -72,131 +44,14 @@ interpretation jctc6: labelledES
     apply(simp only: build_conflict_def) 
     apply(simp add: symmetriccl_def primitive_conflict_def order_def)
     apply(smt numeral_eq_iff semiring_norm(89))
-    apply(rule Transitive_Closure.acyclic_impl_antisym_rtrancl)
-
-
-
-
-
-    using trans_rtrancl apply auto[1]
-      apply (simp add: build_conflict_def symmetric_symmetriccl)
-    apply(simp add: sym_def)
-      apply (meson symm_pc sym_def)
-     apply(simp only: build_conflict_def)
-     apply(simp only: constructed_pc_correct)
-     apply(simp only: constructed_pc_def)
-     apply(simp only: min_order_def)
-      
-     apply(simp only: build_pc_def symmetriccl_def)
-      
-      
-  
-definition jctc6 :: "nat event_structure" where
-"jctc6 \<equiv> \<lparr>
-    event_set = { 1, 2, 3, 4, 5, 6, 7, 8 },
-    primitive_order = { (1, 7), (1, 5), (1, 4), (1, 2), (7, 8), (2, 3), (5, 6) },
-    primitive_conflict =  { (5, 7), (2, 4) },
-    label_function = \<lambda>x.
-        if x = 2 then Label R ''A'' 1 (* r1 *)
-        else if x = 3 then Label W ''B'' 1
-        else if x = 4 then Label R ''A'' 0 (* r1 *)
-        else if x = 5 then Label R ''B'' 1 (* r2 *)
-        else if x = 6 then Label W ''A'' 1
-        else if x = 7 then Label R ''B'' 0 (* r2 *)
-        else if x = 8 then Label W ''A'' 1
-        else Label I '''' 0
-\<rparr>"
-
-definition order :: "nat rel" where
-"order \<equiv> { (6, 6), (3, 3), (1, 8), (1, 7), (1, 6), (1, 5), (1, 4), (1, 3), (1, 2), (1, 1), (8, 8), (7, 8), (7, 7), (2, 3), (2, 2), (4, 4), (5, 6), (5, 5) }"
-
-definition constructed_pc :: "nat rel" where
-"constructed_pc \<equiv> { (2, 4), (4, 2), (5, 7), (7, 5) }"
-
-definition jctc6_expected_results :: "nat set set" where 
-"jctc6_expected_results = { {2, 5} }"
-
-lemma jctc6_acyc_po: "acyclic (primitive_order jctc6)"
-  apply(simp add: jctc6_def)
-  apply(auto)
-        apply(simp add: acyclic_def)
-     (*  apply(rule rtrancl.cases, auto)*)
+  apply(rule Transitive_Closure.acyclic_impl_antisym_rtrancl)
+  apply(simp add: acyclic_def)
+  apply (auto dest!: tranclD) (* thanks to StackOverflow *)
+  (* This proof is a little slow *)
+  apply (smt converse_rtranclE insert_iff num.inject(1) numeral_1_eq_Suc_0 numeral_eq_iff prod.inject 
+          semiring_norm(85) semiring_norm(86) semiring_norm(89) singletonD)+
   done
 
-lemma jctc6_valid_PO: "isValidPO (event_set jctc6) ((primitive_order jctc6)\<^sup>*)"
-  apply(auto simp add: isValidPO_def)
-    apply(rule refl_rtrancl)
-    apply(rule trans_rtrancl)
-  apply(rule acyclic_impl_antisym_rtrancl)
-  apply(simp add: jctc6_acyc_po)
-  done
-
-lemma jctc6_is_finite: "finite (event_set jctc6)"
-  by (simp add: jctc6_def)
-  
-lemma jctc6_symm_conflict: "sym ((symmetriccl (primitive_conflict jctc6))\<^sup>+ - Id)"
-  apply(simp add: sym_def)
-  apply (meson symm_pc sym_def)
-  done
-    
-lemma jctc6_is_conf_valid: "isConfValid ((symmetriccl (primitive_conflict jctc6))\<^sup>+ - Id)"
-  apply(simp add: isConfValid_def jctc6_symm_conflict trans_rtrancl)
-  done
-        
-lemma rtrancl_subset_po: "((primitive_order jctc6)\<^sup>*) \<subseteq> (order \<union> Id)"
-  apply(rule subrelI)
-  apply(rule rtrancl.induct [where ?P = "\<lambda>x y. (x,y) \<in> (order  \<union> Id)"])
-    apply(simp)
-   apply (simp_all add: jctc6_def order_def)
-   apply (smt num.inject(1) num.inject(2) numeral_1_eq_Suc_0 numeral_eq_iff semiring_norm(85) semiring_norm(86) semiring_norm(89))
-  done
-    
-lemma order_sub2: "order \<union> Id \<subseteq> ((primitive_order jctc6)\<^sup>*)"
-  apply(rule subrelI)
-    apply(simp add: order_def jctc6_def)
-  apply auto
-  apply (meson insertI1 insertI2 r_into_rtrancl rtrancl.rtrancl_into_rtrancl)+
-  done
-    
-lemma order_eq_po_order_trancl: "((primitive_order jctc6)\<^sup>*) = order \<union> Id"
-  apply(rule equalityI rtrancl_subset_po order_sub2)+
-  done
-  
-lemma trancl_pc_subset_constructed_pc_id: "((symmetriccl (primitive_conflict jctc6))\<^sup>+) \<subseteq> constructed_pc \<union> Id"
-  apply(rule subrelI)
-  apply(rule trancl.induct [where ?P = "\<lambda>x y. (x,y) \<in> constructed_pc \<union> Id"])
-    apply (simp_all add: jctc6_def constructed_pc_def symmetriccl_def)
-  apply(auto)
-  done
-
-lemma pc_subset_constructed_pc: "((symmetriccl (primitive_conflict jctc6))\<^sup>+ - Id) \<subseteq> constructed_pc"
-  apply(rule alg_subset)
-  apply(rule trancl_pc_subset_constructed_pc_id)
-  done
-    
-lemma constructed_pc_subset_pc: "constructed_pc \<subseteq> ((symmetriccl (primitive_conflict jctc6))\<^sup>+ - Id)"
-  apply(rule subrelI)
-    apply(simp add: symmetriccl_def constructed_pc_def jctc6_def)
-  apply auto
-  done
-    
-lemma constructed_pc_correct: "((symmetriccl (primitive_conflict jctc6))\<^sup>+ - Id) = constructed_pc"
-  apply(rule equalityI constructed_pc_subset_pc pc_subset_constructed_pc)+
-  done
-    
-lemma jctc6_is_minimal: "minimal ((primitive_order jctc6)\<^sup>*) ((symmetriccl (primitive_conflict jctc6))\<^sup>+ - Id)"
-  apply(simp add: minimal_def constructed_pc_correct order_eq_po_order_trancl)
-  apply(simp add: constructed_pc_def order_def)
-  apply (smt num.inject(1) num.inject(2) numeral_1_eq_Suc_0 numeral_eq_iff semiring_norm(85) semiring_norm(86) semiring_norm(89))
-  done
-
-theorem jctc_isValid: "isValidES jctc6"
-  apply(simp add: isValidES_def)
-  apply(simp add: jctc6_is_finite)
-  apply(simp add: jctc6_valid_PO)
-  apply(simp add: jctc6_is_minimal)
-  apply(simp add: jctc6_is_conf_valid)
-  done
 
 definition jctc6_exec:: "nat set" where
   "jctc6_exec \<equiv> {1,2,3,5,6}"
@@ -204,9 +59,25 @@ definition jctc6_exec:: "nat set" where
 definition jctc6_C2:: "nat set" where
   "jctc6_C2 \<equiv> {1,2,3}"
   
-theorem jctc6_reads: "(getMemAction (label_function jctc6 r) = R) = (r \<in> {4,7,2,5})"
-  apply(simp add:jctc6_def)
-  done   
+theorem "jctc6.well_justified jctc6_exec"
+  apply(unfold jctc6.well_justified_def)
+  apply(rule conjI)
+   apply(simp add: jctc6.justified_def)
+   apply(auto simp add: jctc6_exec_def)[1]
+  apply(rule conjI)
+   apply(simp add: jctc6.config_domain_def)
+  apply(rule conjI)
+    apply(simp add: jctc6.conflict_free_def)
+    apply(auto simp add: jctc6.conf_def jctc6.conflict_def)[1]
+    apply(simp add: build_conflict_def)
+    apply(simp add: symmetriccl_def)
+    apply(auto simp add: primitive_conflict_def order_def jctc6_exec_def)[1]
+    try
+    
+  
+theorem jctc6_reads: "(getMemAction (label r) = R) = (r \<in> {4,7,2,5})"
+  apply(simp add: jctc6.label)
+  done
 
 lemma not_read_1[simp]: "\<not>(getMemAction (label_function jctc6 (Suc 0)) = R)"
   apply(simp add: jctc6_def)
@@ -237,43 +108,37 @@ lemma not_read_8[simp]: "\<not> (getMemAction (label_function jctc6 8) = R)"
   apply(simp add: jctc6_def)
   done
     
-lemma write_add_justified: (*"{} \<lesssim>\<^sup>*\<^bsub>es\<^esub> C \<Longrightarrow> 6 \<notin> C' \<and> 8 \<notin> C' \<Longrightarrow> 5 \<in> C \<Longrightarrow> C \<lesssim>\<^sup>*\<^bsub>jctc6\<^esub> C \<union> {6} \<and> (C, C \<union> {6}) \<in> justifies_config jctc6"*)
-  "{} \<lesssim>\<^sup>*\<^bsub>jctc6\<^esub> C' \<Longrightarrow>
-          6 \<notin> C' \<and> 8 \<notin> C' \<Longrightarrow>
-          5 \<in> C' \<Longrightarrow>
-          C' \<lesssim>\<^sup>*\<^bsub>jctc6\<^esub> insert 6 C' \<and>
-          (insert 6 C', jctc6_C2) \<in> justifies_config jctc6"
+lemma write_add_justified:
+  "{} \<lesssim>\<^sup>* C' \<Longrightarrow> 6 \<notin> C' \<and> 8 \<notin> C' \<Longrightarrow> 5 \<in> C' \<Longrightarrow> C' \<lesssim>\<^sup>* insert 6 C' \<and> justifies_config (insert 6 C') jctc6_C2"
   apply (simp add: justifies_config_def)
   apply(rule conjI)
-  apply(insert just_star_imp_just [where es=jctc6, where C'=C'])
+  apply(insert just_star_imp_just [where C'=C'])
     apply(simp)
-  apply(simp add: justifies_config_star_inf_def justifies_config_subset_def justifies_config_inf_def)
-  apply(rule r_into_rtrancl)
-  apply(simp)
-  apply(rule conjI)
+  apply(simp add: justifies_config_star_def justifies_config_subset_def justifies_config_def)
+  apply(rule r_into_rtranclp)
     apply(auto)[1]
   apply (simp add: justifies_config_def is_read_def)
-  apply(auto)[1]
-  apply (simp add: is_read_def)
-  apply(auto simp add: jctc6_def jctc6_C2_def)
+   apply(auto simp add: jctc6_def jctc6_C2_def)
+    try
   done
     
-lemma add_init_justified[simp]: "{} \<lesssim>\<^sup>*\<^bsub>jctc6\<^esub> C \<Longrightarrow> C \<lesssim>\<^sup>*\<^bsub>jctc6\<^esub> C \<union> {1}"
+lemma add_init_justified[simp]: "{} \<lesssim>\<^sup>* C \<Longrightarrow> C \<lesssim>\<^sup>* C \<union> {1}"
   apply (simp add: justifies_config_def)
       apply(insert just_star_imp_just)
-  apply(simp add: justifies_config_star_inf_def justifies_config_subset_def justifies_config_inf_def)
-      apply(rule r_into_rtrancl)
+  apply(simp add: justifies_config_star_def justifies_config_subset_def justifies_config_def)
+      apply(rule r_into_rtranclp)
   apply(simp)
   apply(rule conjI)
     apply(auto)[1]
   apply(simp add: justifies_config_def is_read_def)
   done
-
-lemma add_7_8_justified: "{} \<lesssim>\<^sup>*\<^bsub>jctc6\<^esub> C' \<Longrightarrow> 6 \<notin> C' \<Longrightarrow> 8 \<notin> C' \<Longrightarrow> 5 \<notin> C' \<Longrightarrow>
-   (C' \<union> {1, 7, 8}, jctc6_C2) \<in> justifies_config jctc6"
-  apply(simp add: justifies_config_star_inf_def justifies_config_subset_def justifies_config_inf_def)
-  apply(simp add: justifies_config_def)
-  apply(simp add: jctc6_C2_def jctc6_def)
+    
+  
+lemma add_7_8_justified: "{} \<lesssim>\<^sup>* C' \<Longrightarrow> 6 \<notin> C' \<Longrightarrow> 8 \<notin> C' \<Longrightarrow> 5 \<notin> C' \<Longrightarrow> justifies_config (C' \<union> {1, 7, 8}) jctc6_C2"
+  apply(simp add: justifies_config_star_def justifies_config_subset_def justifies_config_def)
+  apply(simp add: jctc6_C2_def is_read_def)
+    try
+    
   done
 
 lemma justified_7_8: "justified jctc6 {1,7,8}"
@@ -285,8 +150,7 @@ lemma add_1: "{} \<lesssim>\<^sup>*\<^bsub>jctc6\<^esub> C \<Longrightarrow> C \
   apply (simp only: justifies_config_star_inf_def)
   by fastforce
     
-lemma add_7_8_allowed: "{} \<lesssim>\<^sup>*\<^bsub>jctc6\<^esub> C \<Longrightarrow> 6 \<notin> C \<Longrightarrow> 8 \<notin> C \<Longrightarrow> 5 \<notin> C \<Longrightarrow> 
-    C \<lesssim>\<^sup>*\<^bsub>jctc6\<^esub> C \<union> {1, 7, 8}"
+lemma add_7_8_allowed: "{} \<lesssim>\<^sup>* C \<Longrightarrow> 6 \<notin> C \<Longrightarrow> 8 \<notin> C \<Longrightarrow> 5 \<notin> C \<Longrightarrow> C \<lesssim>\<^sup>* C \<union> {1, 7, 8}"
   apply(rule add_1)
     apply(assumption)
    apply(insert just_star_imp_just)
@@ -301,7 +165,7 @@ lemma add_7_8_allowed: "{} \<lesssim>\<^sup>*\<^bsub>jctc6\<^esub> C \<Longright
 text {* We want to case split on C', if C' contains a write from which we can justify 2 then we're 
 good and don't need to add anything to C''. Otherwise we need to add a write like 6 or 8. 
 There's no move for C' which doesn't allow adding 6 or 8 to the C'' set. *}
-theorem round_1: "{} \<sqsubseteq>\<^bsub>jctc6\<^esub> jctc6_C2"
+theorem round_1: "{} \<sqsubseteq> jctc6_C2"
   apply(simp add: ae_justifies_subset_def ae_justifies_def)
   apply (rule allI)
   apply(rule impI)
@@ -487,3 +351,7 @@ theorem "well_justified jctc6 jctc6_exec \<and> {2, 5} \<subseteq> jctc6_exec"
    apply(simp add: jctc6_exec_def)
   apply(simp add: jctc6_exec_def)
   done
+    
+end
+end
+  
