EventStructures2.thy
@@ -4,19 +4,20 @@ begin
 
 datatype mem_action = W | R | I   
 datatype label = Label mem_action string int
-
-type_synonym 'a config = "'a set"
+  
+type_synonym event = nat
+type_synonym 'a config = "event set"
   
 locale partial_order =
-  fixes preceeds :: "'a rel" 
-    and events :: "'a set" ("\<EE>" 1000)
+  fixes preceeds :: "event rel" 
+    and events :: "event set" ("\<EE>" 1000)
   assumes "refl preceeds"
     and "antisym preceeds"
     and "trans preceeds"
 
 locale labelledES = partial_order + 
-  fixes conflict :: "'a rel"
-    and label :: "'a \<Rightarrow> label"
+  fixes conflict :: "event rel"
+    and label :: "event \<Rightarrow> label"
   assumes "sym conflict"
     and confOverPO [intro]: "\<lbrakk> (c, d)\<in>conflict; (d, e)\<in>preceeds \<rbrakk> \<Longrightarrow> (c,e)\<in>conflict"
 
